Trying out "subgoal", and no more [| |]

src/HOL/Auth/OtwayRees.thy
@@ -21,62 +21,62 @@ inductive_set otway :: "event list set"
          (*The spy MAY say anything he CAN say.  We do not expect him to
            invent new nonces here, but he can also use NS1.  Common to
            all similar protocols.*)
- | Fake: "[| evsf \<in> otway;  X \<in> synth (analz (knows Spy evsf)) |]
-          ==> Says Spy B X  # evsf \<in> otway"
+ | Fake: "\<lbrakk>evsf \<in> otway;  X \<in> synth (analz (knows Spy evsf)) \<rbrakk>
+          \<Longrightarrow> Says Spy B X  # evsf \<in> otway"
 
          (*A message that has been sent can be received by the
            intended recipient.*)
- | Reception: "[| evsr \<in> otway;  Says A B X \<in>set evsr |]
-               ==> Gets B X # evsr \<in> otway"
+ | Reception: "\<lbrakk>evsr \<in> otway;  Says A B X \<in>set evsr\<rbrakk>
+               \<Longrightarrow> Gets B X # evsr \<in> otway"
 
          (*Alice initiates a protocol run*)
- | OR1:  "[| evs1 \<in> otway;  Nonce NA \<notin> used evs1 |]
-          ==> Says A B \<lbrace>Nonce NA, Agent A, Agent B,
+ | OR1:  "\<lbrakk>evs1 \<in> otway;  Nonce NA \<notin> used evs1\<rbrakk>
+          \<Longrightarrow> Says A B \<lbrace>Nonce NA, Agent A, Agent B,
                          Crypt (shrK A) \<lbrace>Nonce NA, Agent A, Agent B\<rbrace> \<rbrace>
-                 # evs1 : otway"
+                 # evs1 \<in> otway"
 
          (*Bob's response to Alice's message.  Note that NB is encrypted.*)
- | OR2:  "[| evs2 \<in> otway;  Nonce NB \<notin> used evs2;
-             Gets B \<lbrace>Nonce NA, Agent A, Agent B, X\<rbrace> : set evs2 |]
-          ==> Says B Server
+ | OR2:  "\<lbrakk>evs2 \<in> otway;  Nonce NB \<notin> used evs2;
+             Gets B \<lbrace>Nonce NA, Agent A, Agent B, X\<rbrace> : set evs2\<rbrakk>
+          \<Longrightarrow> Says B Server
                   \<lbrace>Nonce NA, Agent A, Agent B, X,
                     Crypt (shrK B)
                       \<lbrace>Nonce NA, Nonce NB, Agent A, Agent B\<rbrace>\<rbrace>
-                 # evs2 : otway"
+                 # evs2 \<in> otway"
 
          (*The Server receives Bob's message and checks that the three NAs
            match.  Then he sends a new session key to Bob with a packet for
            forwarding to Alice.*)
- | OR3:  "[| evs3 \<in> otway;  Key KAB \<notin> used evs3;
+ | OR3:  "\<lbrakk>evs3 \<in> otway;  Key KAB \<notin> used evs3;
              Gets Server
                   \<lbrace>Nonce NA, Agent A, Agent B,
                     Crypt (shrK A) \<lbrace>Nonce NA, Agent A, Agent B\<rbrace>,
                     Crypt (shrK B) \<lbrace>Nonce NA, Nonce NB, Agent A, Agent B\<rbrace>\<rbrace>
-               : set evs3 |]
-          ==> Says Server B
+               : set evs3\<rbrakk>
+          \<Longrightarrow> Says Server B
                   \<lbrace>Nonce NA,
                     Crypt (shrK A) \<lbrace>Nonce NA, Key KAB\<rbrace>,
                     Crypt (shrK B) \<lbrace>Nonce NB, Key KAB\<rbrace>\<rbrace>
-                 # evs3 : otway"
+                 # evs3 \<in> otway"
 
          (*Bob receives the Server's (?) message and compares the Nonces with
            those in the message he previously sent the Server.
            Need B \<noteq> Server because we allow messages to self.*)
- | OR4:  "[| evs4 \<in> otway;  B \<noteq> Server;
+ | OR4:  "\<lbrakk>evs4 \<in> otway;  B \<noteq> Server;
              Says B Server \<lbrace>Nonce NA, Agent A, Agent B, X',
                              Crypt (shrK B)
                                    \<lbrace>Nonce NA, Nonce NB, Agent A, Agent B\<rbrace>\<rbrace>
                : set evs4;
              Gets B \<lbrace>Nonce NA, X, Crypt (shrK B) \<lbrace>Nonce NB, Key K\<rbrace>\<rbrace>
-               : set evs4 |]
-          ==> Says B A \<lbrace>Nonce NA, X\<rbrace> # evs4 : otway"
+               : set evs4\<rbrakk>
+          \<Longrightarrow> Says B A \<lbrace>Nonce NA, X\<rbrace> # evs4 \<in> otway"
 
          (*This message models possible leaks of session keys.  The nonces
            identify the protocol run.*)
- | Oops: "[| evso \<in> otway;
+ | Oops: "\<lbrakk>evso \<in> otway;
              Says Server B \<lbrace>Nonce NA, X, Crypt (shrK B) \<lbrace>Nonce NB, Key K\<rbrace>\<rbrace>
-               : set evso |]
-          ==> Notes Spy \<lbrace>Nonce NA, Nonce NB, Key K\<rbrace> # evso : otway"
+               : set evso\<rbrakk>
+          \<Longrightarrow> Notes Spy \<lbrace>Nonce NA, Nonce NB, Key K\<rbrace> # evso \<in> otway"
 
 
 declare Says_imp_analz_Spy [dest]
@@ -86,8 +86,8 @@ declare Fake_parts_insert_in_Un  [dest]
 
 
 text\<open>A "possibility property": there are traces that reach the end\<close>
-lemma "[| B \<noteq> Server; Key K \<notin> used [] |]
-      ==> \<exists>evs \<in> otway.
+lemma "\<lbrakk>B \<noteq> Server; Key K \<notin> used []\<rbrakk>
+      \<Longrightarrow> \<exists>evs \<in> otway.
              Says B A \<lbrace>Nonce NA, Crypt (shrK A) \<lbrace>Nonce NA, Key K\<rbrace>\<rbrace>
                \<in> set evs"
 apply (intro exI bexI)
@@ -99,7 +99,7 @@ apply (possibility, simp add: used_Cons)
 done
 
 lemma Gets_imp_Says [dest!]:
-     "[| Gets B X \<in> set evs; evs \<in> otway |] ==> \<exists>A. Says A B X \<in> set evs"
+     "\<lbrakk>Gets B X \<in> set evs; evs \<in> otway\<rbrakk> \<Longrightarrow> \<exists>A. Says A B X \<in> set evs"
 apply (erule rev_mp)
 apply (erule otway.induct, auto)
 done
@@ -108,13 +108,13 @@ done
 (** For reasoning about the encrypted portion of messages **)
 
 lemma OR2_analz_knows_Spy:
-     "[| Gets B \<lbrace>N, Agent A, Agent B, X\<rbrace> \<in> set evs;  evs \<in> otway |]
-      ==> X \<in> analz (knows Spy evs)"
+     "\<lbrakk>Gets B \<lbrace>N, Agent A, Agent B, X\<rbrace> \<in> set evs;  evs \<in> otway\<rbrakk>
+      \<Longrightarrow> X \<in> analz (knows Spy evs)"
 by blast
 
 lemma OR4_analz_knows_Spy:
-     "[| Gets B \<lbrace>N, X, Crypt (shrK B) X'\<rbrace> \<in> set evs;  evs \<in> otway |]
-      ==> X \<in> analz (knows Spy evs)"
+     "\<lbrakk>Gets B \<lbrace>N, X, Crypt (shrK B) X'\<rbrace> \<in> set evs;  evs \<in> otway\<rbrakk>
+      \<Longrightarrow> X \<in> analz (knows Spy evs)"
 by blast
 
 (*These lemmas assist simplification by removing forwarded X-variables.
@@ -132,17 +132,17 @@ NOBODY sends messages containing X!\<close>
 
 text\<open>Spy never sees a good agent's shared key!\<close>
 lemma Spy_see_shrK [simp]:
-     "evs \<in> otway ==> (Key (shrK A) \<in> parts (knows Spy evs)) = (A \<in> bad)"
+     "evs \<in> otway \<Longrightarrow> (Key (shrK A) \<in> parts (knows Spy evs)) = (A \<in> bad)"
 by (erule otway.induct, force,
     drule_tac [4] OR2_parts_knows_Spy, simp_all, blast+)
 
 
 lemma Spy_analz_shrK [simp]:
-     "evs \<in> otway ==> (Key (shrK A) \<in> analz (knows Spy evs)) = (A \<in> bad)"
+     "evs \<in> otway \<Longrightarrow> (Key (shrK A) \<in> analz (knows Spy evs)) = (A \<in> bad)"
 by auto
 
 lemma Spy_see_shrK_D [dest!]:
-     "[|Key (shrK A) \<in> parts (knows Spy evs);  evs \<in> otway|] ==> A \<in> bad"
+     "\<lbrakk>Key (shrK A) \<in> parts (knows Spy evs);  evs \<in> otway\<rbrakk> \<Longrightarrow> A \<in> bad"
 by (blast dest: Spy_see_shrK)
 
 
@@ -151,16 +151,16 @@ subsection\<open>Towards Secrecy: Proofs Involving @{term analz}\<close>
 (*Describes the form of K and NA when the Server sends this message.  Also
   for Oops case.*)
 lemma Says_Server_message_form:
-     "[| Says Server B \<lbrace>NA, X, Crypt (shrK B) \<lbrace>NB, Key K\<rbrace>\<rbrace> \<in> set evs;
-         evs \<in> otway |]
-      ==> K \<notin> range shrK & (\<exists>i. NA = Nonce i) & (\<exists>j. NB = Nonce j)"
+     "\<lbrakk>Says Server B \<lbrace>NA, X, Crypt (shrK B) \<lbrace>NB, Key K\<rbrace>\<rbrace> \<in> set evs;
+         evs \<in> otway\<rbrakk>
+      \<Longrightarrow> K \<notin> range shrK & (\<exists>i. NA = Nonce i) & (\<exists>j. NB = Nonce j)"
 by (erule rev_mp, erule otway.induct, simp_all)
 
 
 (****
  The following is to prove theorems of the form
 
-  Key K \<in> analz (insert (Key KAB) (knows Spy evs)) ==>
+  Key K \<in> analz (insert (Key KAB) (knows Spy evs)) \<Longrightarrow>
   Key K \<in> analz (knows Spy evs)
 
  A more general formula must be proved inductively.
@@ -171,7 +171,7 @@ text\<open>Session keys are not used to encrypt other session keys\<close>
 
 text\<open>The equality makes the induction hypothesis easier to apply\<close>
 lemma analz_image_freshK [rule_format]:
- "evs \<in> otway ==>
+ "evs \<in> otway \<Longrightarrow>
    \<forall>K KK. KK <= -(range shrK) -->
           (Key K \<in> analz (Key`KK Un (knows Spy evs))) =
           (K \<in> KK | Key K \<in> analz (knows Spy evs))"
@@ -182,7 +182,7 @@ apply (drule_tac [5] OR2_analz_knows_Spy, analz_freshK, spy_analz, auto)
 done
 
 lemma analz_insert_freshK:
-  "[| evs \<in> otway;  KAB \<notin> range shrK |] ==>
+  "\<lbrakk>evs \<in> otway;  KAB \<notin> range shrK\<rbrakk> \<Longrightarrow>
       (Key K \<in> analz (insert (Key KAB) (knows Spy evs))) =
       (K = KAB | Key K \<in> analz (knows Spy evs))"
 by (simp only: analz_image_freshK analz_image_freshK_simps)
@@ -190,9 +190,9 @@ by (simp only: analz_image_freshK analz_image_freshK_simps)
 
 text\<open>The Key K uniquely identifies the Server's  message.\<close>
 lemma unique_session_keys:
-     "[| Says Server B \<lbrace>NA, X, Crypt (shrK B) \<lbrace>NB, K\<rbrace>\<rbrace>   \<in> set evs;
+     "\<lbrakk>Says Server B \<lbrace>NA, X, Crypt (shrK B) \<lbrace>NB, K\<rbrace>\<rbrace>   \<in> set evs;
          Says Server B' \<lbrace>NA',X',Crypt (shrK B') \<lbrace>NB',K\<rbrace>\<rbrace> \<in> set evs;
-         evs \<in> otway |] ==> X=X' & B=B' & NA=NA' & NB=NB'"
+         evs \<in> otway\<rbrakk> \<Longrightarrow> X=X' & B=B' & NA=NA' & NB=NB'"
 apply (erule rev_mp)
 apply (erule rev_mp)
 apply (erule otway.induct, simp_all)
@@ -204,8 +204,8 @@ subsection\<open>Authenticity properties relating to NA\<close>
 
 text\<open>Only OR1 can have caused such a part of a message to appear.\<close>
 lemma Crypt_imp_OR1 [rule_format]:
- "[| A \<notin> bad;  evs \<in> otway |]
-  ==> Crypt (shrK A) \<lbrace>NA, Agent A, Agent B\<rbrace> \<in> parts (knows Spy evs) -->
+ "\<lbrakk>A \<notin> bad;  evs \<in> otway\<rbrakk>
+  \<Longrightarrow> Crypt (shrK A) \<lbrace>NA, Agent A, Agent B\<rbrace> \<in> parts (knows Spy evs) -->
       Says A B \<lbrace>NA, Agent A, Agent B,
                  Crypt (shrK A) \<lbrace>NA, Agent A, Agent B\<rbrace>\<rbrace>
         \<in> set evs"
@@ -213,10 +213,10 @@ by (erule otway.induct, force,
     drule_tac [4] OR2_parts_knows_Spy, simp_all, blast+)
 
 lemma Crypt_imp_OR1_Gets:
-     "[| Gets B \<lbrace>NA, Agent A, Agent B,
+     "\<lbrakk>Gets B \<lbrace>NA, Agent A, Agent B,
                   Crypt (shrK A) \<lbrace>NA, Agent A, Agent B\<rbrace>\<rbrace> \<in> set evs;
-         A \<notin> bad; evs \<in> otway |]
-       ==> Says A B \<lbrace>NA, Agent A, Agent B,
+         A \<notin> bad; evs \<in> otway\<rbrakk>
+       \<Longrightarrow> Says A B \<lbrace>NA, Agent A, Agent B,
                       Crypt (shrK A) \<lbrace>NA, Agent A, Agent B\<rbrace>\<rbrace>
              \<in> set evs"
 by (blast dest: Crypt_imp_OR1)
@@ -224,10 +224,10 @@ by (blast dest: Crypt_imp_OR1)
 
 text\<open>The Nonce NA uniquely identifies A's message\<close>
 lemma unique_NA:
-     "[| Crypt (shrK A) \<lbrace>NA, Agent A, Agent B\<rbrace> \<in> parts (knows Spy evs);
+     "\<lbrakk>Crypt (shrK A) \<lbrace>NA, Agent A, Agent B\<rbrace> \<in> parts (knows Spy evs);
          Crypt (shrK A) \<lbrace>NA, Agent A, Agent C\<rbrace> \<in> parts (knows Spy evs);
-         evs \<in> otway;  A \<notin> bad |]
-      ==> B = C"
+         evs \<in> otway;  A \<notin> bad\<rbrakk>
+      \<Longrightarrow> B = C"
 apply (erule rev_mp, erule rev_mp)
 apply (erule otway.induct, force,
        drule_tac [4] OR2_parts_knows_Spy, simp_all, blast+)
@@ -238,9 +238,9 @@ text\<open>It is impossible to re-use a nonce in both OR1 and OR2.  This holds b
   OR2 encrypts Nonce NB.  It prevents the attack that can occur in the
   over-simplified version of this protocol: see \<open>OtwayRees_Bad\<close>.\<close>
 lemma no_nonce_OR1_OR2:
-   "[| Crypt (shrK A) \<lbrace>NA, Agent A, Agent B\<rbrace> \<in> parts (knows Spy evs);
-       A \<notin> bad;  evs \<in> otway |]
-    ==> Crypt (shrK A) \<lbrace>NA', NA, Agent A', Agent A\<rbrace> \<notin> parts (knows Spy evs)"
+   "\<lbrakk>Crypt (shrK A) \<lbrace>NA, Agent A, Agent B\<rbrace> \<in> parts (knows Spy evs);
+       A \<notin> bad;  evs \<in> otway\<rbrakk>
+    \<Longrightarrow> Crypt (shrK A) \<lbrace>NA', NA, Agent A', Agent A\<rbrace> \<notin> parts (knows Spy evs)"
 apply (erule rev_mp)
 apply (erule otway.induct, force,
        drule_tac [4] OR2_parts_knows_Spy, simp_all, blast+)
@@ -249,8 +249,8 @@ done
 text\<open>Crucial property: If the encrypted message appears, and A has used NA
   to start a run, then it originated with the Server!\<close>
 lemma NA_Crypt_imp_Server_msg [rule_format]:
-     "[| A \<notin> bad;  evs \<in> otway |]
-      ==> Says A B \<lbrace>NA, Agent A, Agent B,
+     "\<lbrakk>A \<notin> bad;  evs \<in> otway\<rbrakk>
+      \<Longrightarrow> Says A B \<lbrace>NA, Agent A, Agent B,
                      Crypt (shrK A) \<lbrace>NA, Agent A, Agent B\<rbrace>\<rbrace> \<in> set evs -->
           Crypt (shrK A) \<lbrace>NA, Key K\<rbrace> \<in> parts (knows Spy evs)
           --> (\<exists>NB. Says Server B
@@ -259,9 +259,12 @@ lemma NA_Crypt_imp_Server_msg [rule_format]:
                            Crypt (shrK B) \<lbrace>NB, Key K\<rbrace>\<rbrace> \<in> set evs)"
 apply (erule otway.induct, force,
        drule_tac [4] OR2_parts_knows_Spy, simp_all, blast)
-apply blast  \<comment>\<open>OR1: by freshness\<close>
-apply (blast dest!: no_nonce_OR1_OR2 intro: unique_NA)  \<comment>\<open>OR3\<close>
-apply (blast intro!: Crypt_imp_OR1)  \<comment>\<open>OR4\<close>
+  subgoal \<comment>\<open>OR1: by freshness\<close>
+    by blast  
+  subgoal \<comment>\<open>OR3\<close>
+    by (blast dest!: no_nonce_OR1_OR2 intro: unique_NA)
+  subgoal \<comment>\<open>OR4\<close>
+    by (blast intro!: Crypt_imp_OR1) 
 done
 
 
@@ -270,11 +273,11 @@ text\<open>Corollary: if A receives B's OR4 message and the nonce NA agrees
   bad form of this protocol, even though we can prove
   \<open>Spy_not_see_encrypted_key\<close>\<close>
 lemma A_trusts_OR4:
-     "[| Says A  B \<lbrace>NA, Agent A, Agent B,
+     "\<lbrakk>Says A  B \<lbrace>NA, Agent A, Agent B,
                      Crypt (shrK A) \<lbrace>NA, Agent A, Agent B\<rbrace>\<rbrace> \<in> set evs;
          Says B' A \<lbrace>NA, Crypt (shrK A) \<lbrace>NA, Key K\<rbrace>\<rbrace> \<in> set evs;
-     A \<notin> bad;  evs \<in> otway |]
-  ==> \<exists>NB. Says Server B
+     A \<notin> bad;  evs \<in> otway\<rbrakk>
+  \<Longrightarrow> \<exists>NB. Says Server B
                \<lbrace>NA,
                  Crypt (shrK A) \<lbrace>NA, Key K\<rbrace>,
                  Crypt (shrK B) \<lbrace>NB, Key K\<rbrace>\<rbrace>
@@ -286,28 +289,32 @@ text\<open>Crucial secrecy property: Spy does not see the keys sent in msg OR3
     Does not in itself guarantee security: an attack could violate
     the premises, e.g. by having @{term "A=Spy"}\<close>
 lemma secrecy_lemma:
- "[| A \<notin> bad;  B \<notin> bad;  evs \<in> otway |]
-  ==> Says Server B
+ "\<lbrakk>A \<notin> bad;  B \<notin> bad;  evs \<in> otway\<rbrakk>
+  \<Longrightarrow> Says Server B
         \<lbrace>NA, Crypt (shrK A) \<lbrace>NA, Key K\<rbrace>,
           Crypt (shrK B) \<lbrace>NB, Key K\<rbrace>\<rbrace> \<in> set evs -->
       Notes Spy \<lbrace>NA, NB, Key K\<rbrace> \<notin> set evs -->
       Key K \<notin> analz (knows Spy evs)"
-apply (erule otway.induct, force)
-apply (frule_tac [7] Says_Server_message_form)
-apply (drule_tac [6] OR4_analz_knows_Spy)
-apply (drule_tac [4] OR2_analz_knows_Spy)
-apply (simp_all add: analz_insert_eq analz_insert_freshK pushes)
-apply spy_analz  \<comment>\<open>Fake\<close>
-apply (blast dest: unique_session_keys)+  \<comment>\<open>OR3, OR4, Oops\<close>
-done
+  apply (erule otway.induct, force, simp_all)
+  subgoal \<comment>\<open>Fake\<close>
+    by spy_analz
+  subgoal \<comment>\<open>OR2\<close>
+    by (drule OR2_analz_knows_Spy) (auto simp: analz_insert_eq)
+  subgoal \<comment>\<open>OR3\<close>
+    by (auto simp add: analz_insert_freshK pushes)
+  subgoal \<comment>\<open>OR4\<close>
+    by (drule OR4_analz_knows_Spy) (auto simp: analz_insert_eq)
+  subgoal \<comment>\<open>Oops\<close>
+    by (auto simp add: Says_Server_message_form analz_insert_freshK unique_session_keys)
+  done
 
 theorem Spy_not_see_encrypted_key:
-     "[| Says Server B
+     "\<lbrakk>Says Server B
           \<lbrace>NA, Crypt (shrK A) \<lbrace>NA, Key K\<rbrace>,
                 Crypt (shrK B) \<lbrace>NB, Key K\<rbrace>\<rbrace> \<in> set evs;
          Notes Spy \<lbrace>NA, NB, Key K\<rbrace> \<notin> set evs;
-         A \<notin> bad;  B \<notin> bad;  evs \<in> otway |]
-      ==> Key K \<notin> analz (knows Spy evs)"
+         A \<notin> bad;  B \<notin> bad;  evs \<in> otway\<rbrakk>
+      \<Longrightarrow> Key K \<notin> analz (knows Spy evs)"
 by (blast dest: Says_Server_message_form secrecy_lemma)
 
 text\<open>This form is an immediate consequence of the previous result.  It is 
@@ -318,24 +325,24 @@ to the previous result in that the Spy already has @{term analz} and
 other than Fake are trivial, while Fake requires 
 @{term "Key K \<notin> analz (knows Spy evs)"}.\<close>
 lemma Spy_not_know_encrypted_key:
-     "[| Says Server B
+     "\<lbrakk>Says Server B
           \<lbrace>NA, Crypt (shrK A) \<lbrace>NA, Key K\<rbrace>,
                 Crypt (shrK B) \<lbrace>NB, Key K\<rbrace>\<rbrace> \<in> set evs;
          Notes Spy \<lbrace>NA, NB, Key K\<rbrace> \<notin> set evs;
-         A \<notin> bad;  B \<notin> bad;  evs \<in> otway |]
-      ==> Key K \<notin> knows Spy evs"
+         A \<notin> bad;  B \<notin> bad;  evs \<in> otway\<rbrakk>
+      \<Longrightarrow> Key K \<notin> knows Spy evs"
 by (blast dest: Spy_not_see_encrypted_key)
 
 
 text\<open>A's guarantee.  The Oops premise quantifies over NB because A cannot know
   what it is.\<close>
 lemma A_gets_good_key:
-     "[| Says A  B \<lbrace>NA, Agent A, Agent B,
+     "\<lbrakk>Says A  B \<lbrace>NA, Agent A, Agent B,
                      Crypt (shrK A) \<lbrace>NA, Agent A, Agent B\<rbrace>\<rbrace> \<in> set evs;
          Says B' A \<lbrace>NA, Crypt (shrK A) \<lbrace>NA, Key K\<rbrace>\<rbrace> \<in> set evs;
          \<forall>NB. Notes Spy \<lbrace>NA, NB, Key K\<rbrace> \<notin> set evs;
-         A \<notin> bad;  B \<notin> bad;  evs \<in> otway |]
-      ==> Key K \<notin> analz (knows Spy evs)"
+         A \<notin> bad;  B \<notin> bad;  evs \<in> otway\<rbrakk>
+      \<Longrightarrow> Key K \<notin> analz (knows Spy evs)"
 by (blast dest!: A_trusts_OR4 Spy_not_see_encrypted_key)
 
 
@@ -344,9 +351,9 @@ subsection\<open>Authenticity properties relating to NB\<close>
 text\<open>Only OR2 can have caused such a part of a message to appear.  We do not
   know anything about X: it does NOT have to have the right form.\<close>
 lemma Crypt_imp_OR2:
-     "[| Crypt (shrK B) \<lbrace>NA, NB, Agent A, Agent B\<rbrace> \<in> parts (knows Spy evs);
-         B \<notin> bad;  evs \<in> otway |]
-      ==> \<exists>X. Says B Server
+     "\<lbrakk>Crypt (shrK B) \<lbrace>NA, NB, Agent A, Agent B\<rbrace> \<in> parts (knows Spy evs);
+         B \<notin> bad;  evs \<in> otway\<rbrakk>
+      \<Longrightarrow> \<exists>X. Says B Server
                  \<lbrace>NA, Agent A, Agent B, X,
                    Crypt (shrK B) \<lbrace>NA, NB, Agent A, Agent B\<rbrace>\<rbrace>
                  \<in> set evs"
@@ -358,10 +365,10 @@ done
 
 text\<open>The Nonce NB uniquely identifies B's  message\<close>
 lemma unique_NB:
-     "[| Crypt (shrK B) \<lbrace>NA, NB, Agent A, Agent B\<rbrace> \<in> parts(knows Spy evs);
+     "\<lbrakk>Crypt (shrK B) \<lbrace>NA, NB, Agent A, Agent B\<rbrace> \<in> parts(knows Spy evs);
          Crypt (shrK B) \<lbrace>NC, NB, Agent C, Agent B\<rbrace> \<in> parts(knows Spy evs);
-           evs \<in> otway;  B \<notin> bad |]
-         ==> NC = NA & C = A"
+           evs \<in> otway;  B \<notin> bad\<rbrakk>
+         \<Longrightarrow> NC = NA & C = A"
 apply (erule rev_mp, erule rev_mp)
 apply (erule otway.induct, force,
        drule_tac [4] OR2_parts_knows_Spy, simp_all)
@@ -371,8 +378,8 @@ done
 text\<open>If the encrypted message appears, and B has used Nonce NB,
   then it originated with the Server!  Quite messy proof.\<close>
 lemma NB_Crypt_imp_Server_msg [rule_format]:
- "[| B \<notin> bad;  evs \<in> otway |]
-  ==> Crypt (shrK B) \<lbrace>NB, Key K\<rbrace> \<in> parts (knows Spy evs)
+ "\<lbrakk>B \<notin> bad;  evs \<in> otway\<rbrakk>
+  \<Longrightarrow> Crypt (shrK B) \<lbrace>NB, Key K\<rbrace> \<in> parts (knows Spy evs)
       --> (\<forall>X'. Says B Server
                      \<lbrace>NA, Agent A, Agent B, X',
                        Crypt (shrK B) \<lbrace>NA, NB, Agent A, Agent B\<rbrace>\<rbrace>
@@ -382,24 +389,27 @@ lemma NB_Crypt_imp_Server_msg [rule_format]:
                       Crypt (shrK B) \<lbrace>NB, Key K\<rbrace>\<rbrace>
                     \<in> set evs)"
 apply simp
-apply (erule otway.induct, force,
-       drule_tac [4] OR2_parts_knows_Spy, simp_all)
-apply blast  \<comment>\<open>Fake\<close>
-apply blast  \<comment>\<open>OR2\<close>
-apply (blast dest: unique_NB dest!: no_nonce_OR1_OR2)  \<comment>\<open>OR3\<close>
-apply (blast dest!: Crypt_imp_OR2)  \<comment>\<open>OR4\<close>
+apply (erule otway.induct, force, simp_all)
+  subgoal \<comment>\<open>Fake\<close>
+    by blast 
+  subgoal \<comment>\<open>OR2\<close>
+    by (force dest!: OR2_parts_knows_Spy)
+  subgoal \<comment>\<open>OR3\<close>
+    by (blast dest: unique_NB dest!: no_nonce_OR1_OR2)  \<comment>\<open>OR3\<close>
+  subgoal \<comment>\<open>OR4\<close>
+    by (blast dest!: Crypt_imp_OR2) 
 done
 
 
 text\<open>Guarantee for B: if it gets a message with matching NB then the Server
   has sent the correct message.\<close>
 theorem B_trusts_OR3:
-     "[| Says B Server \<lbrace>NA, Agent A, Agent B, X',
+     "\<lbrakk>Says B Server \<lbrace>NA, Agent A, Agent B, X',
                          Crypt (shrK B) \<lbrace>NA, NB, Agent A, Agent B\<rbrace>\<rbrace>
            \<in> set evs;
          Gets B \<lbrace>NA, X, Crypt (shrK B) \<lbrace>NB, Key K\<rbrace>\<rbrace> \<in> set evs;
-         B \<notin> bad;  evs \<in> otway |]
-      ==> Says Server B
+         B \<notin> bad;  evs \<in> otway\<rbrakk>
+      \<Longrightarrow> Says Server B
                \<lbrace>NA,
                  Crypt (shrK A) \<lbrace>NA, Key K\<rbrace>,
                  Crypt (shrK B) \<lbrace>NB, Key K\<rbrace>\<rbrace>
@@ -410,22 +420,22 @@ by (blast intro!: NB_Crypt_imp_Server_msg)
 text\<open>The obvious combination of \<open>B_trusts_OR3\<close> with 
       \<open>Spy_not_see_encrypted_key\<close>\<close>
 lemma B_gets_good_key:
-     "[| Says B Server \<lbrace>NA, Agent A, Agent B, X',
+     "\<lbrakk>Says B Server \<lbrace>NA, Agent A, Agent B, X',
                          Crypt (shrK B) \<lbrace>NA, NB, Agent A, Agent B\<rbrace>\<rbrace>
            \<in> set evs;
          Gets B \<lbrace>NA, X, Crypt (shrK B) \<lbrace>NB, Key K\<rbrace>\<rbrace> \<in> set evs;
          Notes Spy \<lbrace>NA, NB, Key K\<rbrace> \<notin> set evs;
-         A \<notin> bad;  B \<notin> bad;  evs \<in> otway |]
-      ==> Key K \<notin> analz (knows Spy evs)"
+         A \<notin> bad;  B \<notin> bad;  evs \<in> otway\<rbrakk>
+      \<Longrightarrow> Key K \<notin> analz (knows Spy evs)"
 by (blast dest!: B_trusts_OR3 Spy_not_see_encrypted_key)
 
 
 lemma OR3_imp_OR2:
-     "[| Says Server B
+     "\<lbrakk>Says Server B
               \<lbrace>NA, Crypt (shrK A) \<lbrace>NA, Key K\<rbrace>,
                 Crypt (shrK B) \<lbrace>NB, Key K\<rbrace>\<rbrace> \<in> set evs;
-         B \<notin> bad;  evs \<in> otway |]
-  ==> \<exists>X. Says B Server \<lbrace>NA, Agent A, Agent B, X,
+         B \<notin> bad;  evs \<in> otway\<rbrakk>
+  \<Longrightarrow> \<exists>X. Says B Server \<lbrace>NA, Agent A, Agent B, X,
                             Crypt (shrK B) \<lbrace>NA, NB, Agent A, Agent B\<rbrace>\<rbrace>
               \<in> set evs"
 apply (erule rev_mp)
@@ -438,11 +448,11 @@ text\<open>After getting and checking OR4, agent A can trust that B has been act
   We could probably prove that X has the expected form, but that is not
   strictly necessary for authentication.\<close>
 theorem A_auths_B:
-     "[| Says B' A \<lbrace>NA, Crypt (shrK A) \<lbrace>NA, Key K\<rbrace>\<rbrace> \<in> set evs;
+     "\<lbrakk>Says B' A \<lbrace>NA, Crypt (shrK A) \<lbrace>NA, Key K\<rbrace>\<rbrace> \<in> set evs;
          Says A  B \<lbrace>NA, Agent A, Agent B,
                      Crypt (shrK A) \<lbrace>NA, Agent A, Agent B\<rbrace>\<rbrace> \<in> set evs;
-         A \<notin> bad;  B \<notin> bad;  evs \<in> otway |]
-  ==> \<exists>NB X. Says B Server \<lbrace>NA, Agent A, Agent B, X,
+         A \<notin> bad;  B \<notin> bad;  evs \<in> otway\<rbrakk>
+  \<Longrightarrow> \<exists>NB X. Says B Server \<lbrace>NA, Agent A, Agent B, X,
                                Crypt (shrK B)  \<lbrace>NA, NB, Agent A, Agent B\<rbrace>\<rbrace>
                  \<in> set evs"
 by (blast dest!: A_trusts_OR4 OR3_imp_OR2)
